theories/elpi_prop.v
@@ -11,20 +11,20 @@ Module NurProp (U : Unif).
 
   Lemma size_add_deep l hd tl:
     size (add_deep l hd tl) = size tl.
-  Proof. elim: tl => //=x xs H; rewrite size_cons H//. Qed.
+  Proof. elim: tl => //=-[s x] xs H; rewrite size_cons H//. Qed.
   
   Lemma size_add_ca_deep hd tl:
     size (add_ca_deep hd tl) = size tl.
-  Proof. elim: tl => //=x xs H; rewrite size_cons H//. Qed.
+  Proof. elim: tl => //=-[s x] xs H; rewrite size_cons H//. Qed.
 
   Lemma make_lB0_empty2 {tl} : make_lB0 tl nilC = tl.
-  Proof. rewrite/make_lB0. elim: tl => //=x xs IH; rewrite map_cons cats0 IH//. Qed.
+  Proof. rewrite/make_lB0. elim: tl => //=-[s x] xs IH; rewrite map_cons cats0 IH//. Qed.
 
   Lemma make_lB0_empty1 {lb0} : make_lB0 nilC lb0 = nilC.
   Proof. move=>//. Qed.
 
   Lemma make_lB01_empty2 {tl} : make_lB01 tl nilC = tl.
-  Proof. rewrite/make_lB01. elim: tl => //=x xs IH; rewrite map_cons IH cat0s//. Qed.
+  Proof. rewrite/make_lB01. elim: tl => //=-[s x] xs IH; rewrite map_cons IH cat0s//. Qed.
 
   Lemma make_lB01_empty1 {lb0} : make_lB01 nilC lb0 = nilC.
   Proof. move=>//. Qed.
@@ -39,7 +39,7 @@ Module NurProp (U : Unif).
     { 
       case: l => /=.
         move=>//.
-      move=> x xs; rewrite add_deepG_empty add_deep_empty1//.
+      move=> -[s x] xs; rewrite add_deepG_empty add_deep_empty1//.
     }
     case: x => /=.
       move=>//.
@@ -51,11 +51,12 @@ Module NurProp (U : Unif).
 
   Lemma add_deep_cat bt hd l1 l2: add_deep bt hd (l1 ++ l2) = add_deep bt hd l1 ++ add_deep bt hd l2.
   Proof.
-    elim: l1 l2 bt hd => //= g gs IH l2 bt hd.
+    elim: l1 l2 bt hd => //= -[s g] gs IH l2 bt hd.
     rewrite IH cat_cons//.
   Qed.
   
-  Lemma add_deep_cons bt hd l1 l2: add_deep bt hd (l1 ::: l2) = (add_deepG bt hd l1) ::: (add_deep bt hd l2).
+  Lemma add_deep_cons bt s hd l1 l2: 
+    add_deep bt hd ((s, l1) ::: l2) = (s, add_deepG bt hd l1) ::: (add_deep bt hd l2).
   Proof. move=> //. Qed.
 
   Lemma add_ca_deep_empty2 {tl} : add_ca_deep tl nilC = nilC.
@@ -65,7 +66,7 @@ Module NurProp (U : Unif).
   Lemma add_ca_deep_empty1 {l} : add_ca_deep nilC l = l
     with add_ca_deepG_empty1 {l} : add_ca_deep_goals nilC l = l.
   Proof.
-    { case: l => //= g gs.
+    { case: l => //= -[s g] gs.
       rewrite add_ca_deepG_empty1 add_ca_deep_empty1//.
     }
     case: l => /=.
@@ -75,100 +76,79 @@ Module NurProp (U : Unif).
   Qed.
 
   Section t2l_base.
-    Lemma state_to_list_dead {A l}: is_dead A -> state_to_list A l = nilC.
+    Lemma state_to_list_dead {A l s}: is_dead A -> state_to_list A s l = nilC.
     Proof.
-      elim: A l => //.
-      - move=> A HA s B HB/= l/andP[dA dB]; rewrite HB// HA//.
-      - move=> A HA B0 HB0 B HB l /=dA; rewrite HA//=.
+      elim: A l s => //.
+      - move=> A HA s B HB/= l s1/andP[dA dB]; rewrite HB// HA//.
+      - move=> A HA B0 HB0 B HB l s1 /=dA; rewrite HA//=.
     Qed.
 
-    Lemma base_and_ko_state_to_list {A l}: base_and_ko A -> state_to_list A l = nilC.
+    Lemma base_and_ko_state_to_list {A l s}: base_and_ko A -> state_to_list A s l = nilC.
     Proof. elim: A => //=-[]//. Qed.
 
-    Lemma base_or_aux_ko_state_to_list {A l}: base_or_aux_ko A -> state_to_list A l = nilC.
+    Lemma base_or_aux_ko_state_to_list {A s l}: base_or_aux_ko A -> state_to_list A s l = nilC.
     Proof.
-      elim: A l => //.
-      - move=> /= A HA s B HB l /andP[bA bB]/=; rewrite HB//= base_and_ko_state_to_list//.
+      elim: A l s=> //.
+      - move=> /= A HA s B HB l s1 /andP[bA bB]/=; rewrite HB//= base_and_ko_state_to_list//.
       - move=>[]//.
     Qed.
 
-    Lemma base_and_state_to_list {A}: base_and A -> exists hd, forall l, state_to_list A l = hd ::: nilC.
+    Lemma base_and_state_to_list {A}: base_and A -> exists hd, forall l s, state_to_list A s l = (s, hd) ::: nilC.
     Proof.
       elim: A => //.
       - by eexists.
       - move=> []//p a _ B0 _ B HB/=/andP[/eqP->bB].
         have [hd H]/= := HB bB.
-        case: a => [|t]; eexists => l/=; rewrite H//= !cat0s.
-        rewrite sub0n drop0//.
+        case: a => [|t]; eexists => l s/=; rewrite H//= !cat0s?H//.
+        rewrite sub0n drop0// H//.
     Qed.
 
     Lemma base_and_empty_ca {A B}:
-      base_and A -> (forall l, state_to_list A l = B ::: nilC) -> empty_caG B.
+      base_and A -> (forall l s, state_to_list A s l = (s, B) ::: nilC) -> empty_caG B.
     Proof.
       elim: A B => //=.
-        move=> B _ /(_ nilC) [<-]//.
+        move=> B _ /(_ nilC empty) [<-]//.
       move=> []// p a _ _ _ B HB /=C /andP[/eqP->bB].
       have [hd H]:= base_and_state_to_list bB.
       have:= HB _ bB.
       move=> /(_ _ H) H1.
-      move=> /(_ nilC).
+      move=> /(_ nilC empty).
       rewrite H/=.
       case: a => [|t]/=; rewrite H => [][]<-; rewrite/empty_caG all_cat//.
     Qed.
 
     Lemma bbAnd_state_to_list {A}:
       bbAnd A -> 
-        ((forall l, state_to_list A l = nilC) \/ exists hd, (forall l, state_to_list A l = hd ::: nilC) /\ empty_caG hd).
+        ((forall l s, state_to_list A s l = nilC) \/ 
+          exists hd, (forall l s, 
+            state_to_list A s l = (s, hd) ::: nilC) /\ empty_caG hd).
     Proof.
-      rewrite/bbAnd=>/orP[].
-        move=>/[dup]H/base_and_state_to_list; auto.
-        move=>[hd H1]; right; exists hd.
-        have /= := (base_and_empty_ca H H1).
-        move=> ->; auto.
-      move=>/base_and_ko_state_to_list; auto.
+      rewrite/bbAnd=>/orP[]; last first.
+        move=>/base_and_ko_state_to_list; auto.
+      move=>/[dup]H/base_and_state_to_list; auto.
+      move=>[hd H1]; right; exists hd.
+      have /= := (base_and_empty_ca H H1).
+      move=> ->; auto.
     Qed.
   End t2l_base.
 
   Lemma add_ca_deep_cat l SA SB:
     add_ca_deep l (SA ++ SB) = add_ca_deep l SA ++ add_ca_deep l SB.
-  Proof. elim: SA => //= x xs IH; rewrite IH//. Qed.
+  Proof. elim: SA => //= -[s x] xs IH; rewrite IH//. Qed.
 
-  Lemma success_state_to_list_hd {A} m:
-    success A -> valid_state A ->
-      exists xs, state_to_list A m = nilC ::: xs.
-  Proof.
-    elim: A m => //.
-    - by eexists.
-    - move=> A HA s B HB/= m.
-      case: ifP => [dA sB vB|dA sA /andP[vA bB]].
-        rewrite (state_to_list_dead dA)/=.
-        have [xs {}HB]:= HB nilC sB vB.
-        rewrite HB/=; by eexists.
-      have [xs {}HA]:= HA (state_to_list B nilC) sA vA.
-      rewrite HA; by eexists.
-    - move=> A HA B0 HB0 B HB m /=/andP[sA sB].
-      rewrite sA/=.
-      move=>/and5P[_ vA _ vB bB].
-      have [xs {}HA]:= HA m sA vA; rewrite HA.
-      have [ys HB1]:= HB m sB vB; rewrite HB1.
-      have [H|[hd [H _]]] := bbAnd_state_to_list bB; rewrite H/=; try by eexists.
-      have [zs {}HB]:= HB ((make_lB0 (add_deep m hd xs) hd ++ m)) sB vB; rewrite HB.
-      by eexists.
-  Qed.
-
-  Lemma bbOr_empty_ca B:
-    bbOr B -> empty_ca (state_to_list B nilC).
+  Lemma bbOr_empty_ca B s:
+    bbOr B -> empty_ca (state_to_list B s nilC).
   Proof.
     rewrite/empty_ca.
     rewrite/bbOr=>/orP[]; last first.
       move=>/base_or_aux_ko_state_to_list->//.
-    elim: B => //=.
-    - move=> A HA _ B HB/andP[H1 H2].
+    elim: B s => //=.
+    - move=> A HA s1 B HB s2 /andP[H1 H2].
       rewrite add_ca_deep_empty1 all_cat HB//.
       have [hd H]:= base_and_state_to_list H1.
       rewrite H all_cons.
       rewrite (base_and_empty_ca H1 H)//.
-    - move=> []//=p a _ _ _ B HB/andP[/eqP->]bB.
+    - move=> []//=p a _ _ _ B HB s1 /andP[/eqP->]bB.
       have [hd H]:= base_and_state_to_list bB.
       rewrite H; case: a => [|t]/=; rewrite cats0 H/= /all/=/empty_caG/all/=; 
       have:= (base_and_empty_ca bB H); rewrite /empty_caG/all/= => H1; rewrite H1//.
@@ -184,136 +164,140 @@ Module NurProp (U : Unif).
     case: x H1 => //=-[]//.
   Qed.
 
-  Lemma success_state_to_list {A m}:
+  Lemma is_dead_clean_success {A}:
+    is_dead A = false -> is_dead (clean_success A) = false.
+  Proof.
+    elim: A => //=.
+    - move=> A HA s B HB.
+      case X: is_dead => //=.
+        move=>/HB->; rewrite andbF//.
+      rewrite HA//.
+    - move=> A HA B0 _ B HB dA; rewrite fun_if/= dA if_same//.
+  Qed.
+
+  Lemma success_state_to_list {A s m}:
     valid_state A -> (*we need valid state since in s2l we assume B0 to have length <= 1*)
     success A ->
-      state_to_list A m = nilC ::: (state_to_list (clean_success A) m).
+      state_to_list A s m = (s, nilC) ::: (state_to_list (clean_success A) s m).
   Proof.
-    elim: A m => //.
-    - move=> A HA s B HB/= m.
+    elim: A m s => //.
+    (* - by eexists. *)
+    - move=> A HA s B HB/= m s1.
       case: ifP => [dA vB sB|dA /andP[vA bB] sA].
-        rewrite (state_to_list_dead dA)/=.
-        have:= HB _ vB sB=>->.
-        rewrite !(state_to_list_dead dA)//=.
-      have H //:= HA (state_to_list B nilC) vA sA.
-      rewrite H.
-      move=>/=; f_equal.
-    - move=> A HA B0 HB0 B HB m /= /and5P[oA vA aB] + + /andP[sA sB].
+        rewrite (state_to_list_dead dA) cat0s.
+        have H := HB nilC s1 vB sB.
+        rewrite H/= !(state_to_list_dead dA)//dA//.
+      have H //:= HA (state_to_list B s nilC) s1 vA sA.
+      rewrite H/=is_dead_clean_success//.
+    - move=> A HA B0 HB0 B HB m s1 /= /and5P[oA vA aB] + + /andP[sA sB].
       rewrite sA/==> vB bB.
-      have H1 := HA m vA sA.
-      have H2 := HB m vB sB.
-      rewrite HA//HB//.
+      have H1 := HA m s1 vA sA; rewrite H1/=.
+      have H2 := HB m s1 vB sB; rewrite H2/=.
       have:= bB; rewrite/bbAnd=>/orP[]{}bB; last first.
-        rewrite (base_and_ko_state_to_list bB)//=.
+        by rewrite (base_and_ko_state_to_list bB)//=.
       have [hd H3] := base_and_state_to_list bB.
-      move=>/=.
       rewrite H3/=.
-      remember (state_to_list (clean_success A) _) as cA eqn:HcA.
-      remember (state_to_list (clean_success B) _) as cB eqn:HcB.
-      rewrite -cat_cons; f_equal.
-      remember (make_lB0 _ _).
       rewrite !make_lB01_empty2.
-      apply: HB => //.
+      rewrite -cat_cons; f_equal.
+      set X:= make_lB0 _ _.
+      apply: HB vB sB.
   Qed.
 
   Definition state_to_list_cons A :=
-    forall l, exists x xs, state_to_list A l = x ::: xs.
+    forall m l, exists x xs, state_to_list A m l = x ::: xs.
 
   Section shape.
-    Lemma state_to_list_same_size_aux {r1 r2 A l1 l2}: 
-      state_to_list A l1 = r1 -> state_to_list A l2 = r2 -> size r1 = size r2.
+    Lemma s2l_size {A s1 l1} s2 l2: 
+      size (state_to_list A s1 l1) = size (state_to_list A s2 l2).
     Proof.
-      move=><-<-; clear r1 r2.
-      elim: A l1 l2 => //=.
-        move=> A HA s B HB l1 l2; rewrite !size_add_ca_deep//.
-      move=> A HA B0 HB0 B HB /=l1 l2.
-      have:= HA l1 l2.
-      do 2 case: (state_to_list A) => //=.
-      move=> x xs y ys; rewrite !size_cons => -[]H.
-      have:= HB0 l1 l2.
-      do 2 case: (state_to_list B0) => //=.
-        rewrite !size_map//.
-      move=> w ws z zs; rewrite!size_cons => -[]H1.
-      have:= HB l1 l2.
-      do 2 case: (state_to_list B) => //=.
-        case: zs H1; case: ws; rewrite// !size_cat !size_map !size_add_deep H.
-        move=> _ _; f_equal; apply: HB.
-      move=> t ts r rs; rewrite!size_cons=> -[]H2.
-      case: zs H1; case: ws; rewrite//!size_cat !size_map !size_add_deep H.
-      move=>_; f_equal; apply:HB.
+      elim: A s1 l1 s2 l2 => //=.
+      - move=> p []//.
+      - move=> A HA s B HB s1 l1 s2 l2; rewrite !size_add_ca_deep!size_cat.
+        by f_equal; auto.
+      - move=> A HA B0 HB0 B HB /=s1 l1 s2 l2.
+        have:= HA s1 l1 s2 l2.
+        do 2 case: (state_to_list A) => //=.
+        move=> [s x] xs [s3 y] ys; rewrite !size_cons => -[]H.
+        have:= HB0 s1 l1 s2 l2.
+        do 2 case: (state_to_list B0) => //=.
+          rewrite !size_map//.
+        move=> [s5 w] [|??] [s6 z] [|??]//= _.
+        set X:= make_lB0 _ _.
+        set Y:= make_lB0 _ _.
+        have:= HB s2 (Y++l2) s1 (X++l1) => /(_ _ IsList_alts _ IsList_alts).
+        rewrite !size_cat !size_map !size_add_deep H.
+        move=>->//.
     Qed.
 
-    Lemma state_to_list_empty {A l1 l2}: state_to_list A l1 = nilC -> state_to_list A l2 = nilC.
-    Proof. move=>/state_to_list_same_size_aux => /(_ _ l2 erefl); case: state_to_list => //. Qed.
-
-    Lemma state_to_list_state_to_list_cons {A l x xs}:
-      state_to_list A l = x ::: xs -> state_to_list_cons A.
+    Lemma s2l_empty {A s1 l1 s2 l2}: state_to_list A s1 l1 = nilC -> state_to_list A s2 l2 = nilC.
     Proof.
-      move=> HA l1.
-      have:= state_to_list_same_size_aux HA erefl => /(_ l1).
+      move=> H; have:= f_equal size H => /(_ _ IsList_alts).
+      rewrite (s2l_size s2 l2); case: state_to_list => //.
+    Qed.
+
+    Lemma s2l_cons {A s1 l x xs}:
+      state_to_list A s1 l = x ::: xs -> state_to_list_cons A.
+    Proof.
+      move=> H s2 l2.
+      have:= f_equal size H => /(_ _ IsList_alts).
+      rewrite (s2l_size s2 l2).
       case: state_to_list => //; by do 2 eexists.
     Qed.
 
   End shape.
 
-  Lemma state_to_list_cons_or_fail_right {A s B l}:
-    state_to_list_cons (Or A s B) -> state_to_list B l = nilC -> state_to_list_cons A.
+  Lemma state_to_list_cons_or_fail_right {A s B l s1}:
+    state_to_list_cons (Or A s B) -> 
+      state_to_list B s1 l = nilC -> state_to_list_cons A.
   Proof.
-    move=> HA HB l1.
-    have [y[ys/=]]:= HA l1.
-    rewrite (state_to_list_empty HB)/=cats0.
-    case X: state_to_list => //=.
-    by have:= state_to_list_state_to_list_cons X l1.
-  Qed.
-
-  Lemma state_to_list_cons_and {A B}:
-    state_to_list_cons (And A B B) -> state_to_list_cons A.
-  Proof.
-    move=> HA l1.
-    have [y[ys]]:= HA l1 => /=.
-    case: (state_to_list A) => //; by do 2 eexists.
+    move=> HA HB s2 l2.
+    have [[s3 y][ys/=]]:= HA s1 l.
+    rewrite (s2l_empty HB)/=cats0.
+    case X: state_to_list => [|[s4 g4]gs4]//=[???]; subst.
+    have:= f_equal size X => /(_ _ IsList_alts).
+    rewrite (s2l_size s2 l2).
+    case: state_to_list => //; by do 2 eexists.
   Qed.
 
   Lemma failed_state_to_list {A}:
     valid_state A -> failed A = false -> state_to_list_cons A.
   Proof.
     elim: A => //.
-    - move=> /=. by move=> /=; do 2 eexists.
+    - by move=> /=; do 2 eexists.
     - by move=> /=; do 2 eexists.
     - by move=> p []//=; do 2 eexists.
-    - move=> A HA s B HB/=++l.
+    - move=> A HA s B HB/=++s1 l.
       case: ifP => [dA vB fB|dA /andP[vA bB] fA]/=.
         rewrite (state_to_list_dead dA)/=.
-        have [x[xs H]] := HB vB fB l.
-        have [y[ys ->]]:= state_to_list_state_to_list_cons H nilC.
-        by do 2 eexists.
-      have [x[xs H]] := HA vA fA (state_to_list B l ++ l).
-      have [y[ys ->]]:= state_to_list_state_to_list_cons H (state_to_list B nilC).
+        have [[s2 x][xs H]] := HB vB fB s1 l.
+        have [[s3 hd] [tl]]:= s2l_cons H (if is_dead A then s1 else s) nilC.
+        move=>->/=; by do 2 eexists.
+      set X := state_to_list B _ _.
+      have [[s2 x][xs H]] := HA vA fA s1 X.
+      have [[s3 y][ys ->]]:= s2l_cons H s1 X.
       by do 2 eexists.
-    - move=> A HA B0 _ B HB/= /and5P[oA vA aB]+++l/=.
+    - move=> A HA B0 _ B HB/= /and5P[oA vA aB]+++s1 l/=.
       case: ifP => /=[sA vB bB0|sA /eqP->]/=.
         rewrite success_failed//==>fB.
         rewrite success_state_to_list//.
-        have [x[xs->]]:= HB vB fB l.
+        have [[s2 x][xs->]]:= HB vB fB s1 l.
         move: bB0.
         rewrite /bbOr => /orP[] bB; last first.
           rewrite (base_and_ko_state_to_list bB)/=; by do 2 eexists.
         have [hd H]:= base_and_state_to_list bB.
         rewrite H/=.
         set X:= make_lB0 _ _.
-        have:= HB vB fB (X++l).
-        move=>/(_ _ IsList_alts)[y [ys]]->; by do 2 eexists.
+        have [y[ys->]]:= HB vB fB s1 (X++l).
+        by do 2 eexists.
       rewrite orbF => + fA; rewrite fA => bB.
-      have [x[xs ->]]:= HA vA fA l.
+      have [[s2 x][xs ->]]:= HA vA fA s1 l.
       have fB:= base_and_failed bB.
       have [hd H]:= base_and_state_to_list bB.
       rewrite H/=.
       set X:= make_lB0 _ _.
-      have:= HB (VS.base_and_valid bB) fB (X ++ l).
-      move=>[y[ys->]].
+      have[[s3 y][ys->]]:= HB (VS.base_and_valid bB) fB s1 (X ++ l).
       by do 2 eexists.
   Qed.
-
 
   Lemma next_alt_state_to_list_old {s1 A s2 B}:
     valid_state A -> next_alt s1 A = Some (s2, B) -> state_to_list_cons B.
@@ -332,105 +316,42 @@ Module NurProp (U : Unif).
     valid_state A -> expandedb s A (Done s1 B) b -> state_to_list_cons A.
   Proof. move=> vA /expandedb_Done_not_failed; apply: failed_state_to_list vA. Qed.
 
-  Lemma state_to_list_fail {A s A'}:
-    valid_state A ->
-    expand s A = Failure A' -> state_to_list_cons A' ->
-      state_to_list_cons A.
-  Proof.
-    elim: A s A' => //.
-    - move=> /= _ _ _ [<-]//.
-    - move=>/= p []//.
-    - move=> A HA s B HB s' C/=.
-      case: ifP => //[dA vB|dA /andP[vA bB]] + + l/=.
-        rewrite state_to_list_dead//=.
-        case X: expand => //[D][<-] H1.
-        have [x[xs]]:= H1 l.
-        move=>/=; rewrite (state_to_list_dead dA)/=.
-        case sD: state_to_list => [|w ws]//=[??]; subst.
-        have [x[xs H]] := HB _ _ vB X (state_to_list_state_to_list_cons sD) l.
-        have [y[ys ->]]:= state_to_list_state_to_list_cons H nilC.
-        by do 2 eexists.
-      case X: expand => //[A'][<-] H1.
-      case Z: (state_to_list B) => /=.
-        have H := state_to_list_cons_or_fail_right H1 Z.
-        have [x[xs H2]]:= HA _ _ vA X H l.
-        have [y[ys ->]]:= state_to_list_state_to_list_cons H2 nilC.
-        by do 2 eexists.
-      by case: state_to_list; do 2 eexists.
-    - move=> A HA B0 _ B HB s C /=/and5P[oA vA eB].
-      case X: expand => //[A'|s' A'].
-        rewrite (expand_not_solved_not_success X erefl)/=(expand_failure_failed X).
-        move=> /eqP -> + [<-] + l/= => + /(_ l) [x[xs/=]].
-        rewrite /bbAnd => /orP[]; last first.
-          move=> /base_and_ko_state_to_list->.
-          case sA': state_to_list => [|y ys]//=.
-        move=>/[dup] bB /base_and_state_to_list [hd] H.
-        case sA: state_to_list => [|w ws]//.
-        have [z[zs H1]]:= HA _ _ vA X (state_to_list_state_to_list_cons sA) l.
-        rewrite !H1/= H/=H => -[??]; subst.
-        rewrite H.
-        by do 2 eexists.
-      have [??]:= expand_solved_same X; subst.
-      rewrite (expand_solved_success X)//==> vB bB0.
-      case Y: expand => //[B'][<-] H l/=.
-      have [z[zs]]:= H l => /=.
-      have /= [y[ys ->]] := failed_state_to_list vA (success_failed _ (expand_solved_success X).1) l.
-      move: bB0.
-      rewrite /bbOr => /orP[] bB; last first.
-        rewrite (base_and_ko_state_to_list bB)//=.
-        case sB':state_to_list => [|x xs]//=.
-        move=>[??]; subst.
-        have [z[zs H1]]:= HB _ _ vB Y (state_to_list_state_to_list_cons sB') l.
-        rewrite H1; by do 2 eexists.
-      have [hd H1]:= base_and_state_to_list bB.
-      rewrite /=H1/=.
-      set s1 := state_to_list _ _.
-      set s2 := state_to_list _ _.
-      case sB': s1 => [|w ws]/=.
-        rewrite{1}/make_lB01/=cat0s.
-        move=>->; case: s2; by do 2 eexists.
-      set Z := make_lB0 _ _.
-      have:= HB _ _ vB Y (state_to_list_state_to_list_cons sB') (Z ++ l).
-      move=>[m[ms]]; rewrite/s2.
-      move=>->; by do 2 eexists.
-  Qed.
-
-  Lemma base_or_aux_bot {B}:
-    base_or_aux B -> state_to_list B nilC = nilC -> B = Bot.
+  Lemma base_or_aux_bot {B s1}:
+    base_or_aux B -> state_to_list B s1 nilC = nilC -> B = Bot.
   Proof.
     elim: B => //.
     - move=> A HA s B HB/=/andP[bA bB].
       have [hd ->]// := base_and_state_to_list bA.
     - move=> []//p a _ B0 _ B HB/=/andP[/eqP->]bB.
       have [hd H]// := base_and_state_to_list bB.
-      case: a => [|t]//=; rewrite H/=cats0//.
+      case: a => [|t]//=; rewrite H/=cats0//H//.
   Qed.
 
   Lemma success_success_singleton_next_alt {A l x s}: 
     success A -> valid_state A ->
-      state_to_list A l = x ::: nilC -> next_alt s A = None.
+      state_to_list A s l = x ::: nilC -> next_alt s A = None.
   Proof.
     elim: A l x s=> //.
-    - move=> A HA s B HB l x s1/=.
+    - move=> A HA s B HB l [s2 x] s1/=.
       case: ifP => //[dA sB vB|dA sA /andP[vA]].
         rewrite (state_to_list_dead dA)/=.
-        case SB: state_to_list => //=[z []]//=[?]; subst.
+        case SB: state_to_list => [|[s3 w][|[??]]]//=-[??]; subst.
         rewrite (HB _ _ _ sB vB SB)//.
-      have H := @success_state_to_list _ (state_to_list B nilC) vA sA.
-      have {}H := H _ IsList_alts.
+      have H := success_state_to_list vA sA.
       rewrite H/=.
       move=> bB[]?; subst.
-      case scA: state_to_list => //.
-      case sB: state_to_list => //= _.
-      rewrite (state_to_list_empty scA) in H.
-      rewrite sB in H.
+      case scA: state_to_list => [|[s3 r]rs]//.
+      case sB: state_to_list =>  [|[s4 z]zs]//=? _; subst.
+      rewrite sB in scA.
+      move: H => /(_ s2 no_alt).
+      rewrite scA => H.
       rewrite (HA _ _ _ sA vA H).
       have vB := VS.bbOr_valid bB.
       move: bB.
       rewrite /bbOr => /orP[] bB; last first.
         rewrite next_alt_aux_base_or_ko//if_same//.
       rewrite (base_or_aux_bot bB sB)//.
-    - move=> A HA B0 _ B HB l x s/=/andP[sA sB]/and5P[oA vA aB].
+    - move=> A HA B0 _ B HB l [s1 x] s/=/andP[sA sB]/and5P[oA vA aB].
       rewrite sA/==> vB bB0.
       have H1 := success_state_to_list vA sA.
       have H2 := success_state_to_list vB sB.
@@ -438,45 +359,44 @@ Module NurProp (U : Unif).
       rewrite H1 H2/=.
       move: bB0; rewrite /bbAnd => /orP[].
         move=> /base_and_state_to_list[hd->]/=.
-        set m := make_lB0 _ _.
+        (* set m := make_lB0 _ _. *)
         rewrite H2/= => -[]?.
-        case X: state_to_list => //=; subst.
-        rewrite/m; case Y: state_to_list => //=.
-        have:= H2 (m++l) => /(_ _ IsList_alts); rewrite X => {}H2.
-        have{}H1:= H1 l; rewrite Y in H1.
+        case X: state_to_list => [|[??]?]//=; subst.
+        case Y: state_to_list => [|[]]//=??; subst.
+        move: X; set W := make_lB0 _ _ => X.
+        have:= H2 s1 (W++l) => /(_ _ IsList_alts); rewrite X => {}H2.
+        have{}H1:= H1 s1 l; rewrite Y in H1.
         rewrite (HB _ _ _ sB vB H2) (HA _ _ _ sA vA H1)//.
       move=>/[dup]H /base_and_ko_state_to_list->.
       case X: state_to_list => //=.
       case: x => // _.
-      have:= H2 l; rewrite X => {}H2.
+      have:= H2 s l; rewrite X => {}H2.
       rewrite (HB _ _ _ sB vB H2).
       rewrite base_and_ko_failed//.
       case: next_alt => [[]|]//.
   Qed.
 
-  Lemma state_to_list_empty_clean {B l x}:
+  Lemma state_to_list_empty_clean {B l x s s1}:
     valid_state B ->
-    success B -> state_to_list B l = x ::: nilC ->
-      state_to_list (clean_success B) l = nilC.
+    success B -> state_to_list B s l = x ::: nilC ->
+      state_to_list (clean_success B) s1 l = nilC.
   Proof.
-    move=> H1 H2 H3.
-    have:= @success_state_to_list _ l H1 H2.
-    rewrite H3.
-    case: state_to_list => //.
+    move=> H1 H2; rewrite success_state_to_list//.
+    move=>[] _; apply: s2l_empty.
   Qed.
 
-  Lemma bbOr_next_alt_none {s B l}:
-    bbOr B -> next_alt s B = None -> state_to_list B l = nilC.
+  Lemma bbOr_next_alt_none {s s1 B l}:
+    bbOr B -> next_alt s B = None -> state_to_list B s1 l = nilC.
   Proof.
-    elim: B s l => //.
-    - move=> A HA s B HB s1 l/=; rewrite /bbOr/=.
+    elim: B s s1 l => //.
+    - move=> A HA s B HB s1 s2 l/=; rewrite /bbOr/=.
       move=>/orP[]/andP[bA bB].
         rewrite base_and_dead// next_alt_aux_base_and//.
       rewrite base_and_ko_is_dead// base_or_aux_is_dead//.
       have H1 := @next_alt_aux_base_or_ko _ s bB.
       have H2 :=  @next_alt_aux_base_and_ko _ s1 bA.
-      rewrite (HA _ _ _ H2)// ?(HB _ _ _ H1)///bbOr ?bB?orbT//base_and_ko_base_or_aux_ko//orbT//.
-    - move=> []//p a _ B0 _ B HB s l/=; rewrite /bbOr/=orbF => /andP[/eqP->bB].
+      rewrite (HA _ _ _ _ H2)// ?(HB _ _ _ _ H1)///bbOr ?bB?orbT//base_and_ko_base_or_aux_ko//orbT//.
+    - move=> []//p a _ B0 _ B HB s s1 l/=; rewrite /bbOr/=orbF => /andP[/eqP->bB].
       rewrite next_alt_aux_base_and//.
   Qed.
 
@@ -488,16 +408,16 @@ Module NurProp (U : Unif).
     - move=> A HA s B HB s1 s2 C l/=; rewrite /bbOr/=.
       move=>/orP[]/andP[bA bB].
         rewrite base_and_dead// next_alt_aux_base_and//.
-        move=>[_<-]//.
+        move=>[?<-]//=; subst; rewrite base_and_dead//.
       rewrite base_and_ko_is_dead// base_or_aux_is_dead//.
       rewrite(next_alt_aux_base_or_ko bB) (next_alt_aux_base_and_ko bA)//.
     - move=> []//p a _ B0 _ B HB s1 s2 C l/=; rewrite/bbOr/=orbF => /andP[/eqP->bB].
       rewrite next_alt_aux_base_and// => -[_<-]//.
   Qed.
 
-  Lemma success_next_alt_state_to_list {s1 A l}:
+  Lemma success_next_alt_state_to_list {s1 s2 A l}:
     valid_state A -> success A -> next_alt s1 A = None -> 
-      state_to_list A l = nilC ::: nilC.
+      state_to_list A s2 l = (s2, nilC) ::: nilC.
   Proof.
     elim: A s1 l => //.
     - move=> A HA s B HB s1 l/=.
@@ -510,14 +430,14 @@ Module NurProp (U : Unif).
       case: ifP => dB.
         rewrite valid_state_dead// in H.
       case Y: next_alt => [[]|]// _.
-      have H1 := HA _  (state_to_list B nilC) vA sA X.
+      have H1 := HA _  (state_to_list B s nilC) vA sA X.
       rewrite H1 (bbOr_next_alt_none bB Y)//.
     - move=> A HA B0 _ B HB s1 l /=/and5P[oA vA aB].
       case: ifP => //sA vB/=bB0 sB.
       rewrite success_is_dead// success_failed//.
       case X: next_alt => [[]|]//.
       have {}HB := HB _ _ vB sB X; rewrite HB.
-      case Y: next_alt => [[s2 C]|]//.
+      case Y: next_alt => [[s3 C]|]//.
         move: bB0; rewrite /bbAnd.
         case Z: base_and => //=.
           rewrite base_and_failed//.
@@ -531,58 +451,58 @@ Module NurProp (U : Unif).
       move=>/base_and_ko_state_to_list->//.
   Qed.
 
-  Lemma expand_failure_next_alt_none_empty {A s1 s2 E l}:
+  Lemma expand_failure_next_alt_none_empty {A s1 s2 s3 E l}:
     valid_state A ->
       expand s1 A = Failure E ->
         next_alt s2 E = None ->
-          state_to_list A l = nilC.
+          state_to_list A s3 l = nilC.
   Proof.
-    elim: A s1 s2 E l => //.
+    elim: A s1 s2 s3 E l => //.
     - move=> p []//.
-    - move=> A HA s B HB/=s1 s2 E l.
+    - move=> A HA s B HB/=s1 s2 s3 E l.
       case: ifP => //[dA vB|dA/andP[vA bB]].
         case eB: expand => //[B'][<-]/=.
         rewrite dA.
         case nB': next_alt => [[]|]// _.
-        rewrite (HB _ _ _ _ vB eB nB')/=state_to_list_dead//.
+        rewrite (HB _ _ _ _ _ vB eB nB')/=state_to_list_dead//.
       case eA: expand => //[A'][<-]/=.
       rewrite (expand_not_dead dA eA).
       case nA': next_alt => [[]|]//.
       have vB := VS.bbOr_valid bB.
       rewrite valid_state_dead1//.
       case nB': next_alt => [[]|]// _.
-      rewrite (HA _ _ _ _ vA eA nA')/=.
+      rewrite (HA _ _ _ _ _ vA eA nA')/=.
       move: bB; rewrite /bbOr => /orP[]; last first.
         move=> /base_or_aux_ko_state_to_list->//.
       move=> H; rewrite (next_alt_aux_base_or_none H nB')//.
-    - move=> A HA B0 _ B HB s2 s3 C l/=/and5P[oA vA aB].
+    - move=> A HA B0 _ B HB s2 s3 s4 C l/=/and5P[oA vA aB].
       case eA: expand => //[A'|s' A'].
         have [fA fA']:= expand_failure_failed eA.
         rewrite (failed_success _ fA) fA/==>/eqP->bB[<-]/=.
         rewrite (expand_not_dead (valid_state_dead1 vA) eA)fA'.
-        case nA: next_alt => [[s4 D]|].
+        case nA: next_alt => [[s5 D]|].
           move: bB; rewrite/bbAnd=>/orP[]bB.
             rewrite base_and_failed//.
           rewrite base_and_ko_failed//.
           rewrite (base_and_ko_state_to_list bB)//.
-          case: state_to_list => //=*; rewrite add_alt_empty3//.
-        rewrite (HA _ _ _ _ vA eA nA)//.
+          by case: state_to_list => [|[s6 ?]?]//=.
+        rewrite (HA _ _ _ _ _ vA eA nA)//.
       rewrite (expand_solved_success eA)/= => vB bB0.
       case eB: expand => //[B'][<-]/=.
       have [sA sA'] := expand_solved_success eA.
       rewrite success_is_dead//success_failed//.
       case nB': next_alt => [[]|]//.
-      rewrite (HB _ _ _ _ vB eB (next_alt_none nB' s')).
-      case nA': next_alt => [[s4 D]|]//.
+      rewrite (HB _ _ _ _ _ vB eB (next_alt_none nB' s')).
+      case nA': next_alt => [[s5 D]|]//.
         move: bB0; rewrite/bbAnd=>/orP[]bB.
           rewrite base_and_failed//.
         rewrite base_and_ko_failed//.
         rewrite (base_and_ko_state_to_list bB)//.
-        case: state_to_list => //=*; rewrite add_alt_empty3//.
+        case: state_to_list => [|[]]//.
       rewrite (expand_solved_same eA) (success_next_alt_state_to_list (valid_state_expand vA eA) sA' nA')//.
       case: state_to_list => //=.
-      move=> g []//.
-      rewrite (HB _ _ _ _ vB eB nB')//.
+      move=> [s1 g] []//.
+      rewrite (HB _ _ _ _ _ vB eB nB')//.
   Qed.
 
   Lemma next_alt_propagate_cut {s1 s2 A B}:
@@ -610,399 +530,43 @@ Module NurProp (U : Unif).
   Qed.
 
 
-  Lemma expand_failure_state_to_list_same {s A B l}:
+  Lemma expand_failure_state_to_list_same {s s1 A B l}:
       expand s A = Failure B ->
-          state_to_list A l = state_to_list B l.
+          state_to_list A s1 l = state_to_list B s1 l.
   Proof.
-    elim: A s B l => //.
-    - move=> /= ??? [<-]//.
-    - move=> /= ??? [<-]//.
+    elim: A s s1 B l => //.
+    - move=> /= ???? [<-]//.
+    - move=> /= ???? [<-]//.
     - move=> p [|t]//.
-    - move=> A HA s B HB /= s1 C l.
+    - move=> A HA s B HB /= s1 s2 C l.
       case: ifP => dA.
         case eB: expand => // [B'] [<-]/=.
-        rewrite 2!(state_to_list_dead dA) (HB _ _ _ eB)//.
-      case eA: expand => //[A'][<-]/=.
-      have ->// := HA _ _ _ eA.
-    - move=> A HA B0 _ B HB s C l/=.
+        rewrite 2!(state_to_list_dead dA) (HB _ _ _ _ eB)//dA//.
+      case eA: expand => //[A'][<-]/=; rewrite (expand_not_dead dA eA).
+      have ->// := HA _ _ _ _ eA.
+    - move=> A HA B0 _ B HB s sx C l/=.
       case eA: expand => //[A'|s1 A'].
         have H := expand_failure_failed eA.
         move=> [<-]/=.
-        rewrite (HA _ _ _ eA)//.
+        rewrite (HA _ _ _ _ eA)//.
       have [??] := (expand_solved_same eA); subst.
       case eB: expand => //[B'][<-]/=.
-      case: state_to_list => //x xs.
+      case: state_to_list => //-[s2 x] xs.
       case: state_to_list => //=.
-        rewrite (HB _ _ _ eB)//.
-      move=> y []//; f_equal.
-      rewrite (HB _ _ _ eB)//.
+        rewrite (HB _ _ _ _ eB)//.
+      move=> [s3 y] []//; f_equal.
+      rewrite (HB _ _ _ _ eB)//.
   Qed.
 
-  Lemma base_or_aux_next_alt_some {s B s1 D l}:
-    base_or_aux B -> next_alt s B = Some (s1, D) -> state_to_list B l = state_to_list D l.
+  Lemma base_or_aux_next_alt_some {s B s1 s2 D l}:
+    base_or_aux B -> next_alt s B = Some (s1, D) -> state_to_list B s2 l = state_to_list D s2 l.
   Proof.
-    elim: B s s1 D l => //.
-    - move=>/=???? _[_<-]//.
-    - move=> A HA s B HB s1 s3 C l/=/andP[bA bB].
+    elim: B s s1 s2 D l => //.
+    - move=>/=????? _[_<-]//.
+    - move=> A HA s B HB s1 s2 s3 C l/=/andP[bA bB].
       rewrite base_and_dead//next_alt_aux_base_and//.
-      move=>[_<-]//.
-    - move=> []// p a _ B0 _ B HB s1 s2 C l/=/andP[/eqP->bB].
+      move=>[_<-]//=; rewrite base_and_dead//.
+    - move=> []// p a _ B0 _ B HB s1 s2 s3 C l/=/andP[/eqP->bB].
       rewrite next_alt_aux_base_and// => -[_<-]//.
-  Qed.
-
-  Lemma clean_successP {s1 s2 A B l}:
-    valid_state A -> success A ->
-      next_alt s1 A = Some (s2, B) -> 
-        state_to_list (clean_success A) l = state_to_list B l.
-  Proof.
-    elim: A s1 s2 B l => //.
-    - move=> A HA s B HB s2 s3 C l/=.
-      case: ifP => //[dA vB sB|dA /andP[vA bB] sA].
-        case Y: next_alt => [[s6 E]|]//[_<-]/=.
-        rewrite !(state_to_list_dead dA)/=.
-        rewrite (HB _ _ _ _ vB sB Y)//.
-      case nA: next_alt => [[s6 E]|].
-        move=>[_<-]/=.
-        have ->// := HA _ _ _ _ vA sA nA.
-      case : ifP => //dB.
-      case nB: next_alt => //[[s6 E]][_<-]/=.
-      rewrite (state_to_list_dead is_dead_dead)/=.
-      have H := success_next_alt_state_to_list vA sA nA.
-      have ->/= := state_to_list_empty_clean vA sA (H _).
-      move: bB; rewrite /bbOr => /orP[] bB.
-        have ->// := base_or_aux_next_alt_some bB nB.
-      by rewrite (next_alt_aux_base_or_ko bB) in nB.
-    - move=> A HA B0 _ B HB s2 s3 C l/= /and5P[oA vA eB] + + /andP[sA sB].
-      rewrite sA/==>vB bB0.
-      rewrite success_is_dead//success_failed//.
-      case nB: next_alt => [[s7 E]|].
-        move=>[_<-]/=.
-        rewrite !(success_state_to_list vA sA).
-        have {}HB := (HB _ _ _ _ vB sB nB).
-        rewrite HB//.
-        move: bB0 => /orP[]; last first.
-          move=>/base_and_ko_state_to_list->//.
-        move=>bB.
-        have [h H]:= base_and_state_to_list bB.
-        rewrite H/= HB//.
-      case nA': next_alt => [[s7 A']|]//.
-      case: ifP => // fB0.
-      move=> [??]; subst.
-      move: bB0; rewrite /bbAnd => /orP[bB|]; last first.
-        move=>/base_and_ko_failed; rewrite fB0//.
-      have [x Hb]:= base_and_state_to_list bB.
-      have {}HA := HA _ _ _ _ vA sA nA'. 
-      have H := success_next_alt_state_to_list vB sB nB.
-      rewrite (state_to_list_empty_clean vB sB (H _)).
-      rewrite (success_state_to_list vA sA).
-      rewrite HA Hb/=.
-      have H1 := success_state_to_list vB sB.
-      set m:= make_lB0 _ _.
-      have:= H1 (m ++ l) => /(_ _ IsList_alts).
-      rewrite H.
-      case X: state_to_list => //= _.
-      rewrite Hb/=/m.
-      case Y: state_to_list => [|t ts]//=.
-      rewrite cat0s.
-      rewrite Hb//.
-  Qed.
-
-  Lemma expand_failure_next_alt_state_to_list_cons {s A B s1 s2 C l}:
-    valid_state A -> 
-      expand s A = Failure B ->
-        next_alt s2 B = Some (s1, C) -> 
-          state_to_list A l = state_to_list C l.
-  Proof.
-    elim: A s B s1 s2 C l => //.
-    - move=> /= ??????? [<-]//.
-    - move=> p [|t]//.
-    - move=> A HA s B HB /= s1 C s2 s3 D l.
-      case: ifP => [dA vB|dA /andP[vA bB]].
-        case eB: expand => // [B'] [<-]/=; rewrite dA.
-        case nB': next_alt => [[s4 F]|]//[_<-]/=.
-        rewrite 2!(state_to_list_dead dA) (HB _ _ _ _ _ _ vB eB nB')//.
-      case eA: expand => //[A'][<-]/=; rewrite (expand_not_dead dA eA).
-      case nA': next_alt => [[s4 F]|].
-        move=>[_<-]/=.
-        have ->// := HA _ _ _ _ _ _ vA eA nA'.
-      case: ifP => dB //.
-      case nB: next_alt => //[[s4 F]][_<-].
-      move: bB.
-      rewrite /bbOr; case W: base_or_aux_ko.
-        rewrite next_alt_aux_base_or_ko// in nB.
-      rewrite orbF => bB/=.
-      rewrite (state_to_list_dead is_dead_dead)/=
-        (base_or_aux_next_alt_some bB nB).
-      rewrite (expand_failure_next_alt_none_empty vA eA nA')//.
-    - move=> A HA B0 _ B HB s C/= s2 s3 D l /and5P[oA vA aB].
-      case eA: expand => //[A'|s1 A'].
-        rewrite (expand_not_solved_not_success eA erefl) (expand_failure_failed eA)/=.
-        move=> /eqP-> bB[<-]/=.
-        case: ifP => //dA.
-        rewrite (expand_failure_failed eA).
-        case nA': next_alt => //[[s4 E]].
-        case: ifP => //fB[_<-]/=.
-        move: bB; rewrite /bbAnd.
-        case Z:base_and_ko.
-          rewrite base_and_ko_failed// in fB.
-        rewrite orbF => bB.
-        have [x ->]:= base_and_state_to_list bB.
-        rewrite (HA _ _ _ _ _ _ vA eA nA')//.
-      have [??] := (expand_solved_same eA); subst.
-      have [sA _] := (expand_solved_success eA).
-      rewrite sA/= => vB bB0.
-      rewrite (success_state_to_list vA sA).
-      case eB: expand => //[B'][<-]/=; clear C.
-      rewrite success_is_dead// success_failed//.
-      case nB' : next_alt => [[s4 E]|].
-        move=>[_<-]/=.
-        have [{}s4 {}nB'] := next_alt_some nB' s1.
-        have {}HB := HB _ _ _ _ _ _ vB eB nB'.
-        rewrite (success_state_to_list vA sA)/=.
-        move:bB0 => /orP[]bB; last first.
-          rewrite base_and_ko_state_to_list//HB//.
-        have [hd H]:= base_and_state_to_list bB.
-        have H1 := base_and_empty_ca bB H.
-        rewrite H/= HB//.
-      have H := expand_failure_next_alt_none_empty vB eB nB'.
-      case nA': next_alt => [[s4 E]|]//.
-      case: ifP => //fB0[_<-].
-      move: bB0; rewrite/bbAnd => /orP[]; last first.
-        move=>/base_and_ko_failed; rewrite fB0//.
-      move=> bB0.
-      have [y H1] := base_and_state_to_list bB0.
-      rewrite H1 H/=.
-      have H2 := clean_successP _ sA nA'.
-      rewrite H1 H2//.
-      rewrite make_lB01_empty2 H/= cat0s.
-      case SA: state_to_list => [|x xs]//=.
-      rewrite H1//.
-  Qed.
-
-  Lemma expandedb_failure_next_alt_state_to_list_cons {s1 s2 A B C b1}:
-    valid_state A -> expandedb s1 A (Failed B) b1 -> 
-      next_alt s1 B = Some (s2, C) -> state_to_list_cons C -> 
-        state_to_list_cons A.
-  Proof.
-    remember (Failed _) as f eqn:Hf => + HA.
-    elim: HA s2 B C Hf; clear => //.
-    - move=> s A B HA s1 _ C [<-] vA HB sC l.
-      have [x[xs {}sC]]:= sC l.
-      rewrite (expand_failure_next_alt_state_to_list_cons _ HA HB)// sC.
-      by do 2 eexists.
-    - move=> s s' r A B b HA HB IH s2 C D? vA HC sD; subst.
-      have [{}s2 {}HC]:= next_alt_some HC s'.
-      have{}IH := IH _ _ _ erefl (valid_state_expand vA HA) HC sD.
-      apply: expand_state_to_list_cons vA HA notF.
-    - move=> s s' r A B b HA HB IH s2 C D? vA HC sD; subst.
-      have [{}s2 {}HC]:= next_alt_some HC s'.
-      have{}IH := IH _ _ _ erefl (valid_state_expand vA HA) HC sD.
-      apply: expand_state_to_list_cons vA HA notF.
-  Qed.
-      
-  Lemma runElpi1 A :
-    forall s B s1 b,
-      valid_state A ->
-        runb s A s1 B b -> 
-          state_to_list_cons A.
-  Proof.
-    move=> s B s1 b + H.
-    elim: H; clear.
-    - move=> s s' A B _ b HA _ vA l.
-      apply: expandb_done_state_to_list_cons vA HA _.
-    - move=> s1 s2 _ A B C _ b1 _ _ HA HB _ IH _ vA.
-      have {}IH := IH (valid_state_next_alt (valid_state_expanded vA (ex_intro _ _ HA)) HB).
-      apply: expandedb_failure_next_alt_state_to_list_cons vA HA HB IH.
-  Qed.
-
-
-  Lemma state_to_list_empty_next_alt {B l s2}:
-    valid_state B -> state_to_list B l = nilC ->  next_alt s2 B = None.
-  Proof.
-    elim: B l s2 => //.
-    - move=> p[]//.
-    - move=> A HA s B HB l s2/=.
-      case sA: (state_to_list A) => //=.
-      case sB: (state_to_list B) => //=.
-      case: ifP => //[dA vB|dA /andP[vA bB]].
-        rewrite (HB _ _ vB sB)//.
-      rewrite (HB _ _ (VS.bbOr_valid bB) sB) (HA _ _ vA sA) if_same//.
-    - move=> A HA B0 _ B HB l s2/=/and5P[_ vA _].
-      case: (ifP (is_dead _)) => //dA.
-      case: ifP => /=[sA vB bB0 | sA /eqP->].
-        have [x[xs H]]:= failed_state_to_list vA (success_failed _ sA) l.
-        rewrite H/= success_failed//.
-        move: bB0; rewrite /bbAnd => /orP[] bB0.
-          have [hd H1]:= base_and_state_to_list bB0.
-          rewrite H1/= => Hz.
-          have {Hz}[] := cats20 _ _ Hz.
-          case: xs H => //=H.
-          case sB: state_to_list => [|y ys]//= _ _.
-          rewrite (HB _ _ vB sB) base_and_failed//.
-          by rewrite (success_success_singleton_next_alt sA vA H)//.
-        rewrite (base_and_ko_state_to_list bB0)/=.
-        case sB: state_to_list => [|y ys]//= _.
-        by rewrite (HB _ _ vB sB) base_and_ko_failed//; case: next_alt => [[]|]//.
-      case: ifP => [fA bB|fA bB].
-        case SA: (state_to_list A) => /=[|x xs].
-          by rewrite (HA _ _ vA SA)//.
-        move: bB; rewrite /bbAnd => /orP[]bB.
-          have [hd H]// := base_and_state_to_list bB.
-          by rewrite !H//=!H//.
-        rewrite (base_and_ko_state_to_list bB)/= => _.
-        by rewrite base_and_ko_failed//; case: next_alt => [[]|]//.
-      have [x[xs H]]/= := failed_state_to_list vA fA l.
-      have [hd H1] := base_and_state_to_list bB.
-      rewrite next_alt_aux_base_and//H !H1//=.
-      by rewrite H1//.
-  Qed.
-
-
-  Lemma failed_next_alt_none_state_to_list {s1 A}:
-    valid_state A -> failed A -> next_alt s1 A = None -> 
-      forall l, state_to_list A l = nilC.
-  Proof.
-    elim: A s1 => //.
-    - move=> A HA s B HB s1 /=.
-      case: ifP => [dA vB fB|dA /andP[vA bB] fA].
-        case X: next_alt => [[s2 C]|]//.
-        move=> _ l; rewrite (HB s1)//= state_to_list_dead//.
-      case X: next_alt => [[s2 C]|]//.
-      case: ifP => dB.
-        move=>_ l; rewrite (HA s1)//state_to_list_dead//.
-      (* case: ifP => fB//. *)
-      case Y: next_alt => [[]|]// _ l.
-      rewrite (HA s1)//=.
-      rewrite (bbOr_next_alt_none bB Y)//.
-    - move=> A HA B0 HB0 B HB s1/=/and5P[oA vA aB].
-      case: ifP => /=[sA vB bB0|sA/eqP->].
-        rewrite success_failed//=success_is_dead// => fB.
-        case X: next_alt => [[]|]//.
-        case Y: next_alt => [[s2 C]|]//.
-          case: ifP => fB0// _ l.
-          rewrite (HB s1)//.
-          have:= bB0; rewrite /bbAnd.
-          case Z: base_and => //=.
-            rewrite base_and_failed// in fB0.
-          move=> bB0'.
-          have H := @next_alt_aux_base_and_ko _ empty bB0'.
-          have H1:= bbAnd_valid bB0.
-          rewrite (HB0 empty)//=.
-          by case: state_to_list => //*.
-        move=> _ l.
-        rewrite (success_next_alt_state_to_list vA sA Y) (HB s1)//=.
-        have [->|[hd [-> _]]]//= := bbAnd_state_to_list bB0.
-        by rewrite (HB s1)//=.
-      case: ifP => //fA bB _ + l.
-      case: ifP => //dA.
-        rewrite (state_to_list_dead dA)//.
-      case X: next_alt => [[s2 C]|].
-        case:ifP => fB => //.
-        have:= bB; rewrite /bbAnd.
-        case Z: base_and => //=.
-          rewrite base_and_failed// in fB.
-        move=> bB0'.
-        have H := @next_alt_aux_base_and_ko _ empty bB0'.
-        have H1:= bbAnd_valid bB.
-        rewrite (HB empty)//=; case: state_to_list => //*.
-      have -> //:= HA _ vA fA X l.
-  Qed.
-
-
-  Lemma failed_next_alt_some_state_to_list {s1 A s2 B l}:
-    valid_state A -> failed A -> next_alt s1 A = Some(s2, B) -> 
-      state_to_list A l = state_to_list B l.
-  Proof.
-    elim: A s1 s2 B l => //.
-    - move=> A HA s B HB s1 s2 C l/=.
-      case: ifP => [dA vB fB|dA /andP[vA bB] fA].
-        case X: next_alt => [[s3 D]|]//[_<-]/=.
-        rewrite !(state_to_list_dead dA)//=(HB _ _ _ _ vB fB X)//.
-      case X: next_alt => [[s3 D]|]//.
-        move=>[_<-]/=.
-        rewrite (HA _ _ _ _ vA fA X)//.
-      case: ifP => dB//.
-      case Y: next_alt => [[s3 D]|]//[_<-]/=.
-      rewrite (state_to_list_dead is_dead_dead)/=.
-      rewrite (failed_next_alt_none_state_to_list vA fA X)/=.
-      rewrite (bbOr_next_alt_some bB Y)//.
-    - move=> A HA B0 HB0 B HB s1 s2 C l /=/and5P[oA vA aB].
-      case: (ifP (is_dead _)) => //dA.
-      case: ifP => /=[sA vB bB0|sA/eqP->].
-        rewrite success_failed//= => fB.
-        rewrite (success_state_to_list vA sA)/=.
-        case X: next_alt => [[s3 D]|]//.
-          move=>[_<-]/=.
-          rewrite (success_state_to_list vA sA)/=.
-          have{}HB := (HB _ _ _ _ _ fB X).
-          by have [H|[hd [H M]]]:= bbAnd_state_to_list bB0; rewrite H HB//=HB//.
-        case Y: next_alt => [[s3 D]|]//.
-        move: bB0 => /orP[]bB; last first.
-          rewrite base_and_ko_failed//.
-        rewrite base_and_failed// => -[_<-].
-        have [hd H]:= base_and_state_to_list bB.
-        rewrite H/=!(failed_next_alt_none_state_to_list vB fB X)/=.
-        rewrite (clean_successP vA sA Y).
-        case Z: state_to_list => [|z zs]//=.
-        by rewrite !H//=H//.
-      case: ifP => //fA bB _.
-      case X: next_alt => [[s3 D]|]//.
-      case:ifP => fB => //-[_<-]/=.
-      rewrite (HA _ _ _ _ vA fA X)//.
-  Qed.
-
-  Lemma expand_solved {s A s1 B} l:
-    valid_state A ->
-    expand s A = Success s1 B ->
-    exists x xs,
-      state_to_list A l = x ::: xs /\
-      nur s x xs s1 (state_to_list (clean_success B) l).
-  Proof.
-    move=> vA /[dup] /expand_solved_same [??] H; subst.
-    do 2 eexists; split.
-      apply: success_state_to_list (expand_solved_success H).2.
-      move=>//.
-    apply: StopE.
-  Qed.
-
-  Lemma state_to_list_cutr_empty {A l}:
-    valid_state A -> state_to_list (cutr A) l = nilC.
-  Proof.
-    elim: A l => //.
-    - move=> A HA s B HB l /=; case: ifP => //[dA vB|dA /andP[vA bB]].
-        rewrite HB//state_to_list_dead//is_dead_cutr//.
-      rewrite HA//HB//VS.bbOr_valid//.
-    - move=> A HA B0 _ B HB l /=/and3P[oA vA]; rewrite HA//.
-  Qed.
-
-  Lemma state_to_list_clean_cutl_empty {A l}:
-    valid_state A -> success A -> state_to_list (clean_success (cutl A)) l = nilC.
-  Proof.
-    elim: A l => //.
-    - move=> A HA s B HB l /=; case: ifP => [dA vB sB | dA /andP[vA bB] sA]/=.
-        by rewrite dA/= HB//state_to_list_dead//.
-      by rewrite is_dead_cutl//dA/= HA//state_to_list_cutr_empty//VS.bbOr_valid//.
-    - move=> A HA B0 _ B HB l/=/and5P[oA vA aB] + +/andP[sA sB].
-      rewrite sA success_cut//= => vB bB0.
-      rewrite HB//=.
-      rewrite (success_state_to_list (valid_state_cut sA vA) (success_cut sA))/=.
-      rewrite HA => //.
-      have bB:= bbAnd_cutl bB0.
-      rewrite base_and_ko_state_to_list//.
-  Qed.
-
-  Lemma state_to_list_cutl {A l}:
-    valid_state A -> success A -> state_to_list (cutl A) l = nilC ::: nilC.
-  Proof.
-    elim: A l => //.
-    - move=> A HA s B HB l /=; case: ifP => [dA vB sB | dA /andP[vA bB] sA]/=.
-        rewrite HB//state_to_list_dead//.
-      rewrite (state_to_list_cutr_empty (VS.bbOr_valid bB))/=cats0.
-      rewrite HA//.
-    - move=> A HA B0 _ B HB l/=/and5P[oA vA aB] + +/andP[sA sB].
-      rewrite sA/==> vB bB0.
-      rewrite HA//HB//.
-      have bB:= bbAnd_cutl bB0.
-      rewrite base_and_ko_state_to_list//.
   Qed.
 End NurProp.
