theories/elpi_test.v
@@ -22,239 +22,242 @@ Fixpoint of_goals l :=
 
 Fixpoint of_alt l :=
   match l with
-  | [::] => no_alt
-  | x :: xs => more_alt (of_goals x) (of_alt xs)
+  | [::] => nilC
+  | x :: xs => (empty, of_goals x) ::: (of_alt xs)
   end.
+
+Definition tester l r :=
+  state_to_list l empty nilC = r.
 
 Goal forall B B0 p,
 let f x := (Goal p (Call x)) in
-  state_to_list (And (Or OK empty (f B)) (f B0) Bot) no_alt = 
-    (more_alt (more_goals (call p B) (more_goals (call p B0) no_goals)) no_alt).
+  tester (And (Or OK empty (f B)) (f B0) Bot) 
+    ((empty, (call p B) ::: ((call p B0) ::: nilC)) ::: nilC).
 Proof.
   by move=> //.
 Qed.
 
-Goal forall s1 A B D0 D p,
+Goal forall A B D0 D p,
+  (* (((! \/ A) \/ B)) /\ (D) *)
   let f x := (Goal p (Call x)) in
-  state_to_list 
-    (And (Or ((Or (Goal p Cut) s1 (f A))) s1 (f B)) (f D0) (f D)) no_alt = 
-    of_alt [:: 
+  tester 
+    (And (Or ((Or (Goal p Cut) empty (f A))) empty (f B)) (f D0) (f D)) 
+    (of_alt [:: 
       [::cut (of_alt [:: [:: call p B; call p D0]]); call p D];
       [:: call p A; call p D0]; 
-      [:: call p B; call p D0]].
+      [:: call p B; call p D0]]).
 Proof.
-  move=> s1 A B D0 D p/=.
-  move=>//.
+  move=> A B D0 D p/=.
+  move=>//=.
 Qed.
 
 
-Goal forall s1 s2 B C D E F p,
+Goal forall B C D E F p,
   let f x := (Goal p (Call x)) in
-  (* (A \/_{s1} B) /\_C ((! \/_{s2} D) /\_{E} F) *)
-  state_to_list 
-    (And (Or OK s1 (f B)) (f C) (And (Or (Goal p Cut) s2 (f D)) (f E) (f F))) no_alt = 
-    of_alt [:: 
+  (* (A \/_{empty} B) /\_C ((! \/_{empty} D) /\_{E} F) *)
+  tester 
+    (And (Or OK empty (f B)) (f C) (And (Or (Goal p Cut) empty (f D)) (f E) (f F)))
+    (of_alt [:: 
       [:: cut (of_alt [:: [:: call p B; call p C]]); call p F];
       [:: call p D; call p E]; 
-      [:: call p B; call p C]].
+      [:: call p B; call p C]]).
 Proof.
-  move=> s1 s2 B C D E F p/=.
+  move=> B C D E F p/=.
   rewrite //.
 Qed.
 
 
-Goal forall s1 s2 A B C p,
+Goal forall A B C p,
   let f x := (Goal p (Call x)) in
   (* (((! \/ A) \/ B)) /\ (! \/ C)*)
-  state_to_list 
-    (And (Or ((Or (Goal p Cut) s1 (f A))) s1 (f B)) Bot (Or (Goal p Cut) s2 (f C))) no_alt = 
-    of_alt [:: 
-      [::cut no_alt; cut no_alt];
-      [::cut no_alt; call p C]].
+  tester 
+    (And (Or ((Or (Goal p Cut) empty (f A))) empty (f B)) Bot (Or (Goal p Cut) empty (f C))) 
+    (of_alt [:: 
+      [::cut nilC ; cut nilC ];
+      [::cut nilC ; call p C]]).
 Proof.
-  move=> s1 s2 A B C p/=.
+  move=> A B C p/=.
   rewrite/state_to_list//.
 Qed.
 
-Goal forall s1 s2 A B C0 C p,
+Goal forall A B C0 C p,
   let f x := (Goal p (Call x)) in
   (* (((! \/ A) \/ B)) /\ (! \/ C)*)
-  state_to_list 
-    (And (Or ((Or (Goal p Cut) s1 (f A))) s1 (f B)) (f C0) (Or (Goal p Cut) s2 (f C))) no_alt = 
-    of_alt[:: 
+  tester 
+    (And (Or ((Or (Goal p Cut) empty (f A))) empty (f B)) (f C0) (Or (Goal p Cut) empty (f C)))
+    (of_alt[:: 
       [::cut (of_alt [:: [:: call p B; call p C0]]); cut (of_alt [::[:: call p A; call p C0]; [:: call p B; call p C0]])];
       [::cut (of_alt [:: [:: call p B; call p C0]]); call p C];
       [:: call p A; call p C0]; 
-      [:: call p B; call p C0]].
+      [:: call p B; call p C0]]).
 Proof.
-  move=> s1 s2 A B C0 C p/=.
+  move=> A B C0 C p/=.
   rewrite/state_to_list/=.
   move=>//.
 Qed.
 
 
 
-Goal forall A B0 p s1,
+Goal forall A B0 p,
     (* (OK \/ A) /\_B0 OK *)
   let f x := (Goal p (Call x)) in
-  state_to_list (And (Or OK s1 (f A)) (f B0) OK) no_alt =
-  of_alt [::[::]; [::call p A; call p B0]].
+  tester (And (Or OK empty (f A)) (f B0) OK) (of_alt [::[::]; [::call p A; call p B0]]).
 Proof.
-  move=> A B0 p s1.
+  move=> A B0 p.
   rewrite/state_to_list//=.
 Qed.
 
-Goal forall A B0 p s1,
+Goal forall A B0 p,
   (* (Bot \/ B) /\_b0 B0  *)
   let f x := (Goal p (Call x)) in
-  state_to_list (And (Or Bot s1 (f A)) (f B0) (f B0)) no_alt =
-  of_alt [::[::call p A; call p B0]].
+  tester (And (Or Bot empty (f A)) (f B0) (f B0))
+  (of_alt [::[::call p A; call p B0]]).
 Proof.
-  move=> A B0 p s1.
+  move=> A B0 p.
   rewrite/state_to_list//=.
 Qed.
 
-Goal forall p x y z w s1 s2 a, 
+Goal forall p x y z w a, 
   let f x := (Goal p (Call x)) in
-  state_to_list (
+  tester (
     And 
-      (Or (f x) s1 (f y)) (f a) 
-      (Or (f z) s2 (f w))) no_alt = 
-    of_alt [:: [:: call p x; call p z];
+      (Or (f x) empty (f y)) (f a) 
+      (Or (f z) empty (f w))) 
+    (of_alt [:: [:: call p x; call p z];
     [:: call p x; call p w];
-    [:: call p y; call p a]].
+    [:: call p y; call p a]]).
 Proof.
   move=>/=.
   by [].
 Qed.
 
-Goal forall p z w s1 s2 a, 
+Goal forall p z w a, 
   let f x := (Goal p (Call x)) in
-  state_to_list (
+  tester (
     And 
-      (Or Top s1 Bot) (f a) 
-      (Or (f z) s2 (f w))) no_alt = 
-    of_alt [:: [:: call p z]; [:: call p w]].
+      (Or Top empty Bot) (f a) 
+      (Or (f z) empty (f w))) 
+    (of_alt [:: [:: call p z]; [:: call p w]]).
 Proof.
-  move=>p z w s1 s2 a.
+  move=>p z w a.
   rewrite/state_to_list/=.
   by [].
 Qed.
 
 (* THIS IS IMPORTANT *)
-Goal forall p s1 s2 a b c d, 
+Goal forall p a b c d, 
   let f x := (Goal p (Call x)) in
-  state_to_list (
+  tester (
     And 
-      (Or Bot s1 (f a)) (f b) 
-      (Or (f c) s2 (f d))) no_alt = 
+      (Or Bot empty (f a)) (f b) 
+      (Or (f c) empty (f d))) 
     (* [:: [:: call a; call b] ]. *)
-    of_alt [:: [:: call p a; call p c]; [::call p a; call p d] ].
+    (of_alt [:: [:: call p a; call p c]; [::call p a; call p d] ]).
 Proof.
-  move=> p s1 s2 a b c d /=.
+  move=> p a b c d /=.
   by [].
 Qed.
 
-Goal forall p a b s1 s2, 
+Goal forall p a b, 
 (* (! \/ a) \/ b *)
-  state_to_list (
+  tester (
     Or 
-      (Or (Goal p Cut) s1 (Goal p (Call a))) s2
-      (Goal p (Call b))) no_alt = 
-  of_alt [:: [:: cut (of_alt[:: [:: call p b]])]; [:: call p a]; [:: call p b]].
+      (Or (Goal p Cut) empty (Goal p (Call a))) empty
+      (Goal p (Call b)))
+  (of_alt [:: [:: cut (of_alt[:: [:: call p b]])]; [:: call p a]; [:: call p b]]).
 Proof.
-  move=>p a b s1 s2; rewrite/state_to_list/=.
+  move=>p a b; rewrite/state_to_list/=.
   by []. Qed.
 
 Goal forall A1 A2 s  C0 B p,
   let f x := (Goal p (Call x)) in
-  state_to_list (And (Or (f A1) s (f A2)) (Bot) (And Bot (f C0) (f B))) no_alt =
-  no_alt.
+  tester (And (Or (f A1) s (f A2)) (Bot) (And Bot (f C0) (f B))) nilC
+  .
 Proof.
   move=> A1 A2 s  C0 B p.
   rewrite/state_to_list.
   by [].
 Qed.
 
-Goal forall s A B C p,
+Goal forall A B C p,
   let f x := (Goal p (Call x)) in
-  state_to_list (And (Or (f A) s (f B)) (Bot) (f C)) no_alt =
-  of_alt[:: [:: call p A; call p C]].
+  tester (And (Or (f A) empty (f B)) (Bot) (f C))
+  (of_alt[:: [:: call p A; call p C]]).
 Proof.
   move=> s A B C p.
   rewrite/state_to_list/=.
   by [].
 Qed.
 
-Goal forall A1 A2 s B0 C0 B p,
+Goal forall A1 A2 B0 C0 B p,
   let f x := (Goal p (Call x)) in
-  state_to_list (And (Or (f A1) s (f A2)) (f B0) (And Bot (f C0) (f B))) no_alt =
-  of_alt [:: [:: call p A2 ; call p B0 ]].
+  tester (And (Or (f A1) empty (f A2)) (f B0) (And Bot (f C0) (f B)))
+  (of_alt [:: [:: call p A2 ; call p B0 ]]).
 Proof.
   move=> * /=.
   by [].
 Qed.
 
-Goal forall b0 p a b c s1 s2, 
-  state_to_list (
+Goal forall b0 p a b c, 
+  tester (
     Or 
-      (Or (And (Goal p (Call c)) (Goal p (Call b0)) (Goal p Cut)) s1 (Goal p (Call a))) s2
-      (Goal p (Call b))) no_alt = 
-  of_alt[:: [:: call p c; cut (of_alt[:: [:: call p b]])]; [:: call p a]; [:: call p b]].
+      (Or (And (Goal p (Call c)) (Goal p (Call b0)) (Goal p Cut)) empty (Goal p (Call a))) empty
+      (Goal p (Call b)))
+  (of_alt[:: [:: call p c; cut (of_alt[:: [:: call p b]])]; [:: call p a]; [:: call p b]]).
 Proof.
-  move=> b0 p a b c s1 s2.
+  move=> b0 p a b c.
   rewrite/state_to_list/=.
   rewrite//=.
 Qed.
 
-Goal forall s1 s2 B C Res p,
+Goal forall B C Res p,
   let f x := (Goal p (Call x)) in
   (* (OK \/ B) /\ (! \/ C) -> [cut_[B,Reset]; C; (B, Reset)] *)
-  state_to_list (And (Or OK s1 (f B)) (f Res) (Or (Goal p Cut) s2 (f C))) no_alt
-    = of_alt[::[::cut (of_alt[::[:: call p B; call p Res]])]; [::call p C]; [:: call p B; call p Res]].
+  tester (And (Or OK empty (f B)) (f Res) (Or (Goal p Cut) empty (f C))) 
+    (of_alt[::[::cut (of_alt[::[:: call p B; call p Res]])]; [::call p C]; [:: call p B; call p Res]]).
 Proof.
-  move=> s1 s2 B C Res p.
+  move=> B C Res p.
   rewrite /state_to_list/=.
   move=>//.
 Qed.
 
-Goal forall s1 B C Res Res2 p,
+Goal forall B C Res Reempty p,
   let f x := (Goal p (Call x)) in
   (* (OK \/ B) /\ (! /\ C) -> [cut_[]; C; (B, Reset)] *)
-  state_to_list (And (Or OK s1 (f B)) (f Res) (And (Goal p Cut) (f Res2) (f C))) no_alt
-    = of_alt[::[::cut no_alt; call p C]; [:: call p B; call p Res]].
+  tester (And (Or OK empty (f B)) (f Res) (And (Goal p Cut) (f Reempty) (f C))) 
+    (of_alt[::[::cut nilC; call p C]; [:: call p B; call p Res]]).
 Proof.
-  move=> s1 B C Res Res2 p/=.
+  move=> B C Res Reempty p/=.
   rewrite/state_to_list/=.
   f_equal => //.
 Qed.
 
-Goal forall s1 s2 A B C C0 p,
+Goal forall A B C C0 p,
   let f x := (Goal p (Call x)) in
   (* (A /\ ((! \/ B) \/ C) *)
-  state_to_list (And (f A) (f C0) (Or (Or (Goal p Cut) s1 (f B)) s2 (f C))) no_alt
-  = of_alt [:: 
+  tester (And (f A) (f C0) (Or (Or (Goal p Cut) empty (f B)) empty (f C))) 
+  (of_alt [:: 
     [:: call p A; cut (of_alt[:: [:: call p C]])]; 
     [:: call p A; call p B]; 
-    [:: call p A; call p C]].
+    [:: call p A; call p C]]).
 Proof.
-  move=> s1 s2 A B C C0 p.
+  move=> A B C C0 p.
   rewrite /state_to_list/=.
   repeat f_equal => //.
 Qed.
 
-Goal forall s1 s2 s3 A B C D E p,
+Goal forall A B C D E p,
   let f x := (Goal p (Call x)) in
-  (* (A \/_{s1} B) /\_C ((! \/_{s2} D) \/_{s3} E) *)
-  state_to_list 
-    (And (Or (f A) s1 (f B)) (f C) (Or (Or (Goal p Cut) s2 (f D)) s3 (f E))) no_alt = 
-    of_alt[:: 
+  (* (A \/_{empty} B) /\_C ((! \/_{empty} D) \/_{empty} E) *)
+  tester 
+    (And (Or (f A) empty (f B)) (f C) (Or (Or (Goal p Cut) empty (f D)) empty (f E))) 
+    (of_alt[:: 
     [:: call p A; cut (of_alt [:: [:: call p E]; [:: call p B; call p C]])];
     [:: call p A; call p D]; [:: call p A; call p E];
-    [:: call p B; call p C]]
+    [:: call p B; call p C]])
   .
 Proof.
-  move=> s1 s2 s3 A B C D E p/=.
+  move=> empty A B C D E p/=.
   rewrite/state_to_list/=.
   move=>//.
 Qed.
@@ -266,121 +269,120 @@ Qed.
   The first rejects (D,E) as choice points
   The second rejects (B,C) which is an alternatives at higher level
 *)
-Goal forall s1 s2 B C D E p,
+Goal forall B C D E p,
   let f x := (Goal p (Call x)) in
-  (* (OK \/_{s1} B) /\_C ((! \/_{s2} D) /\_{E} !) *)
-  state_to_list 
-    (And (Or OK s1 (f B)) (f C) (And (Or (Goal p Cut) s2 (f D)) (f E) (Goal p Cut))) no_alt = 
-    of_alt [:: 
-      [:: cut (of_alt[:: [:: call p B; call p C]]); cut no_alt];
+  (* (OK \/_{empty} B) /\_C ((! \/_{empty} D) /\_{E} !) *)
+  tester 
+    (And (Or OK empty (f B)) (f C) (And (Or (Goal p Cut) empty (f D)) (f E) (Goal p Cut))) 
+    (of_alt [:: 
+      [:: cut (of_alt[:: [:: call p B; call p C]]); cut nilC ];
       [:: call p D; call p E]; 
-      [:: call p B; call p C]].
+      [:: call p B; call p C]]).
 Proof.
-  move=> s1 s2 B C D E p/=.
+  move=> B C D E p/=.
   rewrite/state_to_list/=.
   move=>//.
 Qed.
 
-Goal forall s1 s2 A B C p,
+Goal forall A B C p,
   let f x := (Goal p (Call x)) in
   (* ((! \/ ! \/ A) \/ B) \/ C *)
-  state_to_list 
-    (Or (Or (Or (Goal p Cut) s1 ((Or (Goal p Cut) s1 (f A)))) s1 (f B)) s2 (f C)) no_alt = 
-    of_alt[:: 
+  tester
+    (Or (Or (Or (Goal p Cut) empty ((Or (Goal p Cut) empty (f A)))) empty (f B)) empty (f C))
+    (of_alt[:: 
       [::cut (of_alt[:: [:: call p B]; [::call p C]])];
       [::cut (of_alt[:: [:: call p B]; [::call p C]])];
       [:: call p A]; 
       [:: call p B];
-      [:: call p C] ].
+      [:: call p C] ]).
 Proof.
-  move=> s1 s2 A B C p/=.
+  move=> A B C p/=.
   rewrite/state_to_list/=.
   move=>//=.
 Qed.
 
-Goal forall s1 s2 A B C p,
+Goal forall A B C p,
   let f x := (Goal p (Call x)) in
   (* ((! \/ ! \/ A) \/ B) \/ C *)
-  state_to_list 
-    (Or (Or (Or (And (Goal p Cut) Top Top) s1 ((Or (Goal p Cut) s1 (f A)))) s1 (f B)) s2 (f C)) no_alt = 
-    of_alt[:: 
+  tester 
+    (Or (Or (Or (And (Goal p Cut) Top Top) empty ((Or (Goal p Cut) empty (f A)))) empty (f B)) empty (f C)) 
+    (of_alt[:: 
       [::cut (of_alt[:: [:: call p B]; [::call p C]])];
       [::cut (of_alt[:: [:: call p B]; [::call p C]])];
       [:: call p A]; 
       [:: call p B];
-      [:: call p C] ].
+      [:: call p C] ]).
 Proof.
-  move=> s1 s2 A B C p/=.
+  move=> A B C p/=.
   rewrite/state_to_list/=.
   move=>//=.
 Qed.
 
 
-Goal forall s1 s2 A B C D0 D p,
+Goal forall A B C D0 D p,
   let f x := (Goal p (Call x)) in
   (* (((! \/ ! \/ A) \/ B) \/ C) /\ D*)
-  state_to_list 
-    (And (Or (Or (Or (Goal p Cut) s1 ((Or (Goal p Cut) s1 (f A)))) s1 (f B)) s2 (f C)) (f D0) (f D)) no_alt = 
-    of_alt[:: 
+  tester
+    (And (Or (Or (Or (Goal p Cut) empty ((Or (Goal p Cut) empty (f A)))) empty (f B)) empty (f C)) (f D0) (f D))
+    (of_alt[:: 
       [::cut (of_alt [:: [:: call p B; call p D0]; [::call p C; call p D0]]); call p D];
       [::cut (of_alt [:: [:: call p B; call p D0]; [::call p C; call p D0]]); call p D0];
       [:: call p A; call p D0]; 
       [:: call p B; call p D0];
-      [:: call p C; call p D0] ].
+      [:: call p C; call p D0] ]).
 Proof.
-  move=> s1 s2 A B C D0 D p/=.
+  move=> A B C D0 D p/=.
   rewrite/state_to_list/=.
   f_equal => //.
 Qed.
 
-Goal forall X s1 s2 A B C D0 D p,
+Goal forall X A B C D0 D p,
   let f x := (Goal p (Call x)) in
   (* ((X \/ ((! \/ ! \/ A) \/ B) \/ C)) /\ D*)
-  state_to_list 
-    (And (Or (f X) s1 (Or (Or (Or (Goal p Cut) s1 ((Or (Goal p Cut) s1 (f A)))) s1 (f B)) s2 (f C))) (f D0) (f D)) no_alt = 
-    of_alt[:: 
+  tester 
+    (And (Or (f X) empty (Or (Or (Or (Goal p Cut) empty ((Or (Goal p Cut) empty (f A)))) empty (f B)) empty (f C))) (f D0) (f D))
+    (of_alt[:: 
       [:: call p X; call p D];
       [::cut (of_alt[:: [:: call p B; call p D0]; [::call p C; call p D0]]); call p D0];
       [::cut (of_alt[:: [:: call p B; call p D0]; [::call p C; call p D0]]); call p D0];
       [:: call p A; call p D0]; 
       [:: call p B; call p D0];
-      [:: call p C; call p D0] ].
+      [:: call p C; call p D0] ]).
 Proof.
-  move=> X s1 s2 A B C D0 D p/=.
+  move=> X A B C D0 D p/=.
   rewrite/state_to_list/=.
   f_equal => //.
 Qed.
 
-
-Goal forall s1 s2 B0 A B C D p,
+Goal forall B0 A B C D p,
   let f x := (Goal p (Call x)) in
   (* (((A /\ (! \/ B)) \/ C \/ D)) *)
-  state_to_list 
-    (Or (Or (f C) s2 (And (f A) (f B0) (Or (Goal p Cut) s1 (f B)))) s1 (f D)) no_alt = 
-    of_alt[:: 
+  tester 
+    (Or (Or (f C) empty (And (f A) (f B0) (Or (Goal p Cut) empty (f B)))) empty (f D))
+    (of_alt[:: 
       [:: call p C]; 
       [:: call p A; cut (of_alt[:: [:: call p D]])]; 
-      [:: call p A; call p B]; [:: call p D]].
+      [:: call p A; call p B]; [:: call p D]]).
 Proof.
-  move=> s1 s2 B0 A B C D p/=.
+  move=> B0 A B C D p/=.
   rewrite/state_to_list/=.
   rewrite//.
 Qed.
 
-Goal forall s1 s2 s3 s4 p A B C,
+Goal forall p A B C,
   let f x := (Goal p (Call x)) in
   (* (((! \/ A) \/ !) \/ B) \/ C *)
-  state_to_list 
-    (Or (Or (Or (Or (Goal p Cut) s1 (f A)) s2 (Goal p Cut)) s3 (f B)) s4 (f C)) no_alt = 
-    of_alt[:: 
+  tester 
+    (Or (Or (Or (Or (Goal p Cut) empty (f A)) empty (Goal p Cut)) empty (f B)) empty (f C))
+    (of_alt[:: 
       [::cut (of_alt[::[::cut (of_alt[::[::call p B]; [::call p C]])]; [::call p B]; [::call p C]])];
       [::call p A];
       [::cut (of_alt[::[::call p B]; [::call p C]])];
       [::call p B];
       [::call p C]
-    ].
+    ]).
 Proof.
-  move=> s1 s2 s3 s4 p A B C/=.
+  move=> p A B C/=.
   rewrite/state_to_list/=.
   rewrite//.
 Qed.
@@ -388,8 +390,8 @@ Qed.
 Goal forall p l,
   let s := ((Or (Or Dead empty (Goal p Cut)) empty Top)) in
   let bt := of_alt([::] :: l) in
-  state_to_list s (of_alt l) = of_alt[:: [:: cut bt]; [::]] /\ 
-    state_to_list (clean_success (get_state (expand empty s))) (of_alt l) ++ (of_alt l) = bt.
+  state_to_list s empty (of_alt l) = of_alt[:: [:: cut bt]; [::]] /\ 
+    state_to_list (clean_success (get_state (expand empty s))) empty (of_alt l) ++ (of_alt l) = bt.
 Proof.
   simpl get_state.
   move=>//=.
